rocq-osiris/examples/proofs/shiftreset.v
@@ -24,9 +24,8 @@ Section shift_protocol.
 
   Definition is_shift (Ψ : iEff Σ) (Φ Q : val → iPropO Σ) h : iProp Σ :=
     iSpec τ[cont] h (λ k m,
-        ∀ ι,
-        (∀ w, Q w -∗ EWP[ι] (resume k (O2Ret w)) <| Ψ |> {{ ensures v, Φ v }}) -∗
-        ▷ EWP[ι] m <| Ψ |> {{ ensures v, Φ v }})%I.
+        (∀ w, Q w -∗ may_resume (O2Ret w) k ⊤ Ψ ⊥ Φ) -∗
+        ▷ imp m <| Ψ |> {{ Φ }})%I.
 
   (* Note that this specification is different from in [Hazel]; there is
      no recursive reference within the specification itself. *)
@@ -34,15 +33,15 @@ Section shift_protocol.
   Definition SHIFT ℓ :
     (iEffO -d> (val -d> iPropO Σ) -d> iEffO) := λ Ψ Φ,
     (>> h Q >> !(shift ℓ h) {{ (is_shift Ψ Φ Q h) }};
-      << w << ?(w) {{ Q ↑ w }} @ OS)%ieff.
+      << w << ?(O2Ret w) {{ Q w }})%ieff.
 
   Lemma upcl_SHIFT ℓ Ψ Φ v Φ' :
-    iEff_car (upcl OS (SHIFT ℓ Ψ Φ)) v Φ' ≡
+    (SHIFT ℓ Ψ Φ) allows perform v << Φ' >> ⊣⊢
       (∃ t Q,
           ⌜v = shift ℓ t ⌝ ∗ is_shift Ψ Φ Q t ∗
-          (∀ w, Q ↑ w -∗ Φ' w))%I.
+          (∀ v, Q v -∗ Φ' (O2Ret v)))%I.
   Proof.
-    transitivity (iEff_car (upcl OS (SHIFT ℓ Ψ Φ)) v Φ').
+    transitivity (iEff_car (upcl (SHIFT ℓ Ψ Φ)) v Φ').
     - by iApply iEff_car_proper.
     - by rewrite /SHIFT (upcl_tele' [tele _ _] [tele _]).
   Qed.
@@ -64,16 +63,24 @@ Section reasoning_rules.
   Definition reset_spec ℓ : val → microvx → iProp Σ :=
     λ f m,
       (∀ (Ψ : iEff Σ) (Φ : val → iProp Σ),
-          iSpec τ[unit] f (λ _ m, EWP m <|SHIFT ℓ Ψ Φ|> {{ ensures v, Φ v }}) -∗
-          EWP m <|Ψ|> {{ ensures v, Φ v }})%I.
+          iSpec τ[unit] f (λ _ m, imp m <|SHIFT ℓ Ψ Φ|> {{ Φ }}) -∗
+          imp m <|Ψ|> {{ Φ }})%I.
 
   Definition shift_spec ℓ : val → microvx → iProp Σ :=
     λ f m,
       (∀ (Ψ : iEff Σ) (Φ Q : val → iProp Σ),
           is_shift Ψ Φ Q f -∗
-          EWP m <|SHIFT ℓ Ψ Φ|> {{ ensures v, Q v}})%I.
+          imp m <|SHIFT ℓ Ψ Φ|> {{ Q }})%I.
 
 End reasoning_rules.
+
+Inductive effect : Type :=
+| Shift (f : val).
+
+Local Instance encode_effect l : Encode effect :=
+  { encode := λ eff, match eff with
+                     | Shift f => VXData l [f]
+                     end }.
 
 (* ------------------------------------------------------------------------ *)
 (** Verification. *)
@@ -81,220 +88,85 @@ End reasoning_rules.
 Section verification.
   Context `{!osirisGS Σ}.
 
-  Lemma ewp_ensures_val {X} ι (Φ : val → iProp Σ) (m : micro val X) E Ψ :
-    EWP[ι] m @ E <|Ψ|> {{ ensures #v, Φ v }} ⊣⊢ EWP[ι] m @ E <|Ψ|> {{ ensures v, Φ v }}.
-  Proof.
-    iStartProof; iSplit; iIntros "Hwp"; iApply (ewp_mono with "Hwp");
-      (iIntros ([|]); [ | iIntros ([]) ]).
-    - iIntros "(%v & -> & $)".
-    - iIntros "HΦ". iExists a.
-      iSplit; [ equality | iAssumption ].
-  Qed.
+  Context (shift_eff : loc).
+  Local Instance : Encode effect := encode_effect shift_eff.
 
-  Lemma establish_shift_spec η (shift_eff : loc) :
+  Lemma establish_shift_spec η :
     lookup_name η "Shift" = ret (VLoc shift_eff) →
-    ⊢ EWP eval η (EAnonFun __fun0)
-      {{ ensures v, □ iSpec τ[val] v (shift_spec shift_eff) }}.
+    ⊢ imp eval η (EAnonFun __fun0)
+      {{ λ v, □ iSpec τ[val] v (shift_spec shift_eff) }}.
   Proof.
-    iIntros (Hlookup ι).
-    iApply (ewp_EAnon_pers τ[val]); simpl.
+    iIntros (henc Hlookup).
+    iApply (imp_EAnon_pers τ[val]); simpl.
     iIntros "!>" (f). rewrite /shift_spec.
-    iIntros (Ψ Φ Q) "Hf %ι'".
-    iApply ewp_please; iNext.
-    iApply (ewp_EPerform _ _ _ _ (λ v, ⌜v = VXData shift_eff [f]⌝)%I).
-    { simpl_eval. rewrite Hlookup /widen /try /=. iApply prove_ewp_Par.
-      iApply ewp_ret. instantiate (1 := (λ v, ⌜v = f⌝)%I). equality.
-      iApply ewp_ret. instantiate (1 := (λ v, ⌜v = []⌝)%I). equality.
-      iIntros (?? -> ->) "/=".
-      iApply ewp_ret. equality. }
+    iIntros (Ψ Φ Q) "Hf".
+    iApply imp_please; iNext.
+    iApply (imp_EPerform (λ eff, ⌜eff = Shift f⌝)%I).
+    { iApply imp_EXData. apply Hlookup. instantiate (1:=[(λ v, ⌜v = f⌝)]%I).
+      iApply big_sepL2_singleton.
+      iApply imp_EPath. iApply imp_ret; first encode. auto.
+      iIntros (vs) "Hvs".
+      iPoseProof (big_sepL2_length with "Hvs") as "%Hlen".
+      destruct vs; first discriminate; destruct vs; last discriminate.
+      simpl; iDestruct "Hvs" as "[-> _]".
+      iExists _; iSplit; [ iPureIntro | equality ].
+      reflexivity. }
     iIntros (? ->).
-    iApply ewp_perform.
-    rewrite /prot upcl_SHIFT. iFrame.
+    rewrite upcl_SHIFT. iFrame.
     iSplit; first equality.
-    iIntros (o) "$".
+    iIntros (o) "$". auto.
   Qed.
 
-  Lemma establish_reset_spec η (shift_eff : loc) :
+  Lemma establish_reset_spec η :
     lookup_name η "Shift" = ret (VLoc shift_eff) →
-    ⊢ EWP eval η (EAnonFun __fun2)
-      {{ ensures v, □ iSpec τ[val] v (reset_spec shift_eff) }}.
+    ⊢ imp eval η (EAnonFun __fun2)
+      {{ λ v, □ iSpec τ[val] v (reset_spec shift_eff) }}.
   Proof.
-    iIntros (Hlookup ι).
-    iApply (ewp_EAnon_pers τ[val]); simpl.
+    iIntros (henc Hlookup).
+    iApply (imp_EAnon_pers τ[val]); simpl.
     iIntros "!>" (f). rewrite /reset_spec.
-    iIntros (Ψ Φ) "Hf %ι'".
-    iApply ewp_please; iNext.
+    iIntros (Ψ Φ) "Hf".
+    iApply imp_please; iNext.
 
-    iApply ewp_EMatch.
-
-    iApply (ewp_deep_handler _ _ (SHIFT shift_eff Ψ Φ) (Φ ↑) with "[Hf]").
-    { iApply (ewp_mono with "[-]").
-      iApply (ewp_EApp τ[unit] with "[Hf]").
-      simpl_eval. iApply ewp_ret. iApply "Hf".
-      simpl_eval. iApply ewp_ret. instantiate (1 := (λ u, ⌜u = tt⌝)%I). equality; encode.
-      simpl. iIntros (? -> m) "Hwp".
-      iApply (ewp_mono with "Hwp").
-      iIntros ([|]); [ | iIntros ([]) ]. simpl.
-      iIntros "!> HΦ". iExists a. rewrite <- solve_encode_val. iSplit; [ equality | iExact "HΦ" ].
-      iIntros ([|]); [ | iIntros ([]) ]. simpl.
-      iIntros "(%v &-> & $)". }
+    iApply (imp_EHandler with "[Hf]").
+    { iApply (imp_EApp τ[unit] with "[Hf]").
+      { iApply imp_EPath. iApply imp_ret; first encode.
+        iApply "Hf". }
+      { iApply imp_EConstant; first encode.
+        instantiate (1 := (λ u, ⌜u = tt⌝)%I). done. }
+      simpl. iIntros (?) "-> %m $". }
 
     iLöb as "IH".
-    iApply prove_deep_handler_spec; iSplit.
+    iApply prove_deep_handler_spec.
+    iSplit; last (iSplit; first iIntros (? [])).
 
     (* Base case: we just return the value. *)
-    { iIntros (?). iIntros "H !>"; destruct o; try done.
-      next_branch.
-      iIntros (? ->).
-      iApply ewp_EPath. by iApply ewp_ret. }
+    { iIntros (v) "Φ !>".
+      iApply deep_handle_cons. iPureIntro. ltac2:(specify_cpattern ()). pattern_match.
+      iSplit; [ iIntros (? ->) | iIntros ([]) ].
+      iApply imp_EPath. iApply (imp_ret with "Φ"); encode. }
 
     (* Handler case: an effect is being performed. *)
-    iIntros (v k) "Hprot"; rewrite /prot.
+    iIntros (v k) "Hprot".
     rewrite upcl_SHIFT.
     iDestruct "Hprot" as (g Q) "[-> [Hg Hk]]".
-    rewrite /deep_handler_spec seal_eq.
 
     unfold is_shift.
 
-    iModIntro.
-    next_branch. iIntros (? []).
-    next_branch. iIntros (? ->).
-    iApply ewp_ensures_val.
-    iApply (ewp_EApp τ[cont] with "[Hg] []").
-    simpl_eval. iApply ewp_ret. iAssumption.
-    simpl_eval. iApply ewp_ret. instantiate (1 := (λ v, ⌜v = k⌝)%I). iExists k; equality.
-    iIntros (? -> m) "Hwp". rewrite /tapp.
-    iApply ewp_ensures_val.
+    iModIntro. iApply deep_handle_cons. iPureIntro; ltac2:(specify_cpattern ()).
+    iSplit; [ iIntros (? []) | iIntros (_) ].
+    iApply deep_handle_cons. iPureIntro; ltac2:(specify_cpattern ()). pattern_match.
+    iSplit; [ iIntros (? ->) | iIntros (Hf); tauto ].
+    iApply (imp_EApp τ[cont] with "[Hg] []").
+    { iApply imp_EPath. iApply imp_ret; first encode. iApply "Hg". }
+    { iApply imp_EPath. iApply imp_ret; first encode.
+      instantiate (1 := (λ v, ⌜v = k⌝)%I). done. }
+    iIntros (? -> m) "Hwp".
     iApply "Hwp".
     iIntros (v) "HQ".
-    iSpecialize ("Hk" $! (O2Ret v) with "HQ").
-    iApply "Hk". iNext.
-    iApply "IH".
-    tauto.
+    iApply ("Hk" with "HQ IH").
   Qed.
 
   Definition dummy_env := ("Effect", VStruct [("Deep", VStruct [])]) :: stdlib_env.
-
-  Lemma module_proof :
-    ⊢ EWP (eval_mexpr dummy_env __main)
-      {{ ensures v, ∃ η, ⌜v = VStruct η⌝ ∧ ⌜lookup_name η "main" = ret #4⌝ }}.
-  Proof.
-    iIntros (ι).
-    iApply ewp_module.
-    iApply (ewp_sitems_cons _ _ _ (ieq ?[φ])).
-
-    (* [open Effect] *)
-    { iApply (ewp_sitem_open _ _ (ieq ?[φ3])).
-      { simpl_eval_mexpr. iApply ewp_ret. equality. }
-      iIntros (δ' ->). equality. }
-
-    (* [open Effect.Deep] *)
-    iIntros (? ->).
-    iApply (ewp_sitems_cons _ _ _ (ieq ?[φ])); [ | iIntros (? ->)].
-    { iApply (ewp_sitem_open _ _ (ieq ?[φ2]));
-        [ | iIntros (? ->); equality ].
-      simpl_eval_mexpr. iApply ewp_ret. equality. }
-
-    (* [type _ Effect.t += Shift : t Effect.t] *)
-    iApply ewp_sitems_extend.
-    iIntros ([η δ]) "(%shift_eff & -> & Hshifteff)"; clear η δ.
-
-    (* [let shift f = perform (Shift f)] *)
-    iApply (ewp_sitems_let_singleton_var (λ v, □ iSpec τ[val] v (shift_spec shift_eff))%I).
-    { iApply establish_shift_spec; auto. }
-    iIntros ([η δ]) "(%shift & -> & #Hshift)". clear η δ.
-
-    (* [let reset f = try f () with ...] *)
-    iApply (ewp_sitems_let_singleton_var (λ v, □ iSpec τ[val] v (reset_spec shift_eff))%I).
-    { iApply establish_reset_spec; auto. }
-    iIntros ([η δ]) "(%reset & -> & #Hreset)". clear η δ.
-
-    (* [let main = reset (fun _ -> ...)] *)
-    iApply (ewp_sitems_let_singleton_var (λ v, ⌜v = #4⌝)%I with "[Hshift Hreset]").
-    { (* Change the postcondition to [ensures #n, ⌜n = 4%Z⌝]. *)
-      iApply (ewp_mono with "[-]"); last first.
-      { instantiate (1 := (ensures #n, ⌜n = 4%Z⌝)%I).
-        iIntros ([|]); [ | iIntros ([]) ].
-        iIntros "(%v & -> & ->)". equality. }
-
-      (* Prove that [reset (fun _ -> ...)] return [n = 4]. *)
-      iApply (ewp_EApp τ[val] with "[Hreset] [Hshift]").
-      { simpl_eval. iApply ewp_ret. iAssumption. }
-      2: { simpl.
-           iIntros (v) "Hv %m reset_spec".
-           unfold reset_spec, tapp. iNext.
-           iApply ("reset_spec" with "Hv"). }
-
-      iApply ewp_ensures_val.
-      iApply (ewp_EAnon τ[unit]).
-      iIntros ([] ι').
-      iApply (ewp_please); iNext.
-      (* [fun _ -> ...] gets translated to [match anon with | _ -> ...] *)
-      iApply ewp_EMatch.
-      iApply (ewp_deep_handler).
-      { simpl_eval. iApply ewp_ret. instantiate (1 := (ensures #v, ⌜v = tt⌝)%I).
-        iExists tt; equality. }
-      iApply prove_deep_handler_spec.
-      iSplit; last first.
-      { instantiate (1 := ⊥).
-        iIntros (??); rewrite /prot upcl_bottom; iIntros ([]). }
-      iIntros ([|]); [ | iIntros ([]) ].
-      iIntros "(%u & -> & ->) !>".
-
-      iApply deep_handle_cons; [ iPureIntro | iSplit ].
-      {  ltac2:(specify_cpattern ()). pattern_match. apply eq_refl. }
-      2: { iIntros ([]). }
-      iIntros (? <-).
-
-      (* Subgoal: [shift (fun k -> ...) + 3] returns [4]. *)
-      iApply (ewp_EIntAdd); clear ι.
-      { (* Prove that [shift (fun k -> ...)] returns [1]? *)
-        iApply (ewp_EApp τ[val]).
-        { simpl_eval. iApply ewp_ret. iAssumption. }
-        2: { iIntros (f) "Hf %m shift_spec".
-             unfold shift_spec, tapp.
-             iNext.
-             iApply ("shift_spec" with "Hf"). }
-
-        rewrite ewp_ensures_val.
-        iApply (ewp_EAnon τ[cont]); simpl.
-
-        iIntros (k ι) "Hresume".
-        iApply ewp_please; iIntros "!> !>".
-        (* Subgoal: [continue k 0 + 1] retuns [4]. *)
-        iApply (ewp_EIntAdd with "[Hresume]").
-        { iApply ewp_EContinue'.
-          { (* Evaluate [k]. *)
-            simpl_eval. iApply ewp_ret.
-            instantiate (1 := (λ v, ⌜v = k⌝)%I). iExists _; equality. }
-          { (* Evalutate [0]. *)
-            simpl_eval. iApply ewp_ret.
-            instantiate (1 := (λ v, ⌜v = #0%Z⌝)%I). equality. }
-          iIntros (? ? -> ->).
-          iApply "Hresume".
-          instantiate (1 := (λ v, ⌜v = 0%Z⌝)%I).
-          iExists 0%Z; equality. }
-        { (* Evaluate [1]. *)
-          iApply (ewp_EInt with "[]").
-          instantiate (1 := (λ n, ⌜n = 1%Z⌝)%I). iExists _; equality. }
-        iIntros (n1 n2) "(-> & ->)". equality.
-        (* The goal is now [(4 + 1) = 4]. *)
-        admit. }
-      { (* Evaluate [3]. *)
-        iApply ewp_EInt.
-        instantiate (1 := (λ n, ⌜n = 3⌝)%I). iExists _ ; equality. }
-
-      iIntros (n1 n2) "(-> & ->)".
-      (* The goal is now [(0 + 3) = 4]*)
-      admit. }
-
-    iIntros ([η δ]) "(%main & -> & %Hres)".
-
-    iApply ewp_sitems_nil. simpl.
-    iExists _. iSplit; first equality.
-    iPureIntro.
-    simpl. rewrite Hres. reflexivity.
-
-  Admitted.
 
 End verification.
